Intermediate/CSInvariants.v
@@ -1,0 +1,78 @@
+Require Import CompCert.Events.
+Require Import CompCert.Smallstep.
+Require Import CompCert.Behaviors.
+Require Import Common.Definitions.
+Require Import Common.Util.
+Require Import Common.Linking.
+Require Import Common.Memory.
+Require Import Common.Reachability.
+Require Import Common.Renaming.
+Require Import Common.Traces.
+Require Import Common.TracesInform.
+Require Import Common.CompCertExtensions.
+Require Import Intermediate.Machine.
+Require Import Intermediate.GlobalEnv.
+Require Import Intermediate.CS.
+Require Import Lib.Extra.
+Require Import Lib.Monads.
+
+From mathcomp Require Import ssreflect eqtype ssrfun.
+From mathcomp Require ssrbool.
+From extructures Require Import fmap fset.
+
+Set Bullet Behavior "Strict Subproofs".
+
+Module CSInvariants.
+
+Import Intermediate.
+
+  
+Definition is_prefix (s: CS.state) (p: program) t : Prop :=
+  Star (CS.sem_non_inform p) (CS.initial_machine_state p) t s.
+
+Inductive wf_ptr_wrt_cid_t (cid: Component.id) (t: trace event) : Pointer.t -> Prop
+  :=
+  | wf_ptr_own:
+      forall p b o,
+        wf_ptr_wrt_cid_t cid t (p, cid, b, o)
+  | wf_ptr_shared:
+      forall p c_other b o,
+      addr_shared_so_far (c_other, b) t -> wf_ptr_wrt_cid_t cid t (p, c_other, b, o)
+.
+
+Inductive wf_load_wrt_t_pc
+          (mem: Memory.t)
+          (load_at: Pointer.t)
+          (t: trace event)
+          (pc: Pointer.t) : Pointer.t -> Prop :=
+| wrt_load_ptr_wf_load:
+    forall ptr,
+      wf_ptr_wrt_cid_t (Pointer.component load_at) t ptr ->
+      wf_load_wrt_t_pc mem load_at t pc ptr
+| wrt_pc_wf_load:
+    forall ptr,
+      addr_shared_so_far (Pointer.component load_at, Pointer.block load_at) t ->
+      wf_ptr_wrt_cid_t (Pointer.component pc) t ptr ->
+      wf_load_wrt_t_pc mem load_at t pc ptr.
+        
+Definition wf_mem_wrt_t_pc (mem: Memory.t) (t: trace event) (pc: Pointer.t) : Prop :=
+  forall load_at ptr,
+    Memory.load mem load_at = Some (Ptr ptr) ->
+    wf_load_wrt_t_pc mem load_at t pc ptr.
+
+Definition wf_reg_wrt_t_pc (reg: Register.t) (t: trace event) (pc: Pointer.t) : Prop :=
+  forall r ptr,
+    Register.get r reg = Ptr ptr ->
+    wf_ptr_wrt_cid_t (Pointer.component pc) t ptr.
+
+Definition wf_state_t (s: CS.state) (t: trace event) : Prop :=
+  wf_mem_wrt_t_pc (CS.state_mem s) t (CS.state_pc s) /\
+  wf_reg_wrt_t_pc (CS.state_regs s) t (CS.state_pc s).
+
+Lemma is_prefix_wf_state_t s p t:
+  well_formed_program p ->
+  is_prefix s p t ->
+  wf_state_t s t.
+Admitted.
+  
+End CSInvariants.
